Typing hints for Dargent

cogent/Main.hs
@@ -725,7 +725,7 @@ parseArgs args = case getOpt' Permute options args of
             tpthy  = thy ++ suf
         writeFileMsg tpfile
         output tpfile $ flip LJ.hPutDoc $
-          deepTypeProof id __cogent_ftp_with_decls __cogent_ftp_with_bodies tpthy nfed' log
+          deepTypeProof id __cogent_ftp_with_decls __cogent_ftp_with_bodies tpthy nfed' fts log
       shallowTypeNames <-
         genShallow cmds source stg nfed' typedefs fts log (Shallow stg `elem` cmds,
                                                            SCorres stg `elem` cmds,
@@ -796,7 +796,7 @@ parseArgs args = case getOpt' Permute options args of
             let tpfile = mkThyFileName source __cogent_suffix_of_type_proof
                 tpthy  = mkProofName source (Just __cogent_suffix_of_type_proof)
             writeFileMsg tpfile
-            output tpfile $ flip LJ.hPutDoc $ deepTypeProof id __cogent_ftp_with_decls __cogent_ftp_with_bodies tpthy monoed' log
+            output tpfile $ flip LJ.hPutDoc $ deepTypeProof id __cogent_ftp_with_decls __cogent_ftp_with_bodies tpthy monoed' fts log
           when (AllRefine `elem` cmds) $ do
             let arfile = mkThyFileName source __cogent_suffix_of_all_refine
             writeFileMsg arfile
@@ -950,7 +950,7 @@ parseArgs args = case getOpt' Permute options args of
     genDeep cmds source stg defns typedefs fts log = do
       let dpfile = mkThyFileName source (__cogent_suffix_of_deep ++ __cogent_suffix_of_stage stg)
           thy = mkProofName source (Just $ __cogent_suffix_of_deep ++ __cogent_suffix_of_stage stg)
-          de = deep thy stg defns log
+          de = deep thy stg defns fts log
       putProgressLn ("Generating deep embedding (" ++ stgMsg stg ++ ")...")
       writeFileMsg dpfile
       output dpfile $ flip LJ.hPutDoc de
