cogent/src/Cogent/Inference.hs
@@ -23,7 +23,6 @@
 {-# LANGUAGE KindSignatures #-}
 {-# LANGUAGE LambdaCase #-}
 {-# LANGUAGE MultiWayIf #-}
-{-# LANGUAGE PartialTypeSignatures #-}
 {-# LANGUAGE PatternGuards #-}
 {-# LANGUAGE PolyKinds #-}
 {-# LANGUAGE Rank2Types #-}
@@ -60,6 +59,7 @@ import Control.Monad.State hiding (fmap, forM_)
 import Control.Monad.Trans.Maybe
 import Data.Foldable (forM_)
 import Data.Function (on)
+import Data.List (nub)
 import qualified Data.IntMap as IM
 import Data.Map (Map)
 import Data.Maybe (isJust)
@@ -233,28 +233,28 @@ substituteL _  t                 = t
 substituteS :: [DataLayout BitRange] -> Sigil (DataLayout BitRange) -> Sigil (DataLayout BitRange)
 substituteS ls Unboxed = Unboxed
 substituteS ls (Boxed b CLayout) = Boxed b CLayout
-substituteS ls (Boxed b (Layout l)) = Boxed b . Layout $ substituteS' ls l
-  where
-    substituteS' :: [DataLayout BitRange] -> DataLayout' BitRange -> DataLayout' BitRange
-    substituteS' ls l = case l of
-      VarLayout n s -> case ls !! (natToInt n) of
-                       CLayout -> __impossible "substituteS in Inference: CLayout shouldn't be here"
-                       Layout l -> offset s l
-      SumLayout tag alts ->
-        let altl = M.toList alts
-            fns = fmap fst altl
-            fis = fmap fst $ fmap snd altl
-            fes = fmap snd $ fmap snd altl
-         in SumLayout tag $ M.fromList (zip fns $ zip fis (fmap (substituteS' ls) fes))
-      RecordLayout fs ->
-        let fsl = M.toList fs
-            fns = fmap fst fsl
-            fes = fmap snd fsl
-         in RecordLayout $ M.fromList (zip fns (fmap (substituteS' ls) fes))
+substituteS ls (Boxed b (Layout l)) = Boxed b . Layout $ substituteDL ls l
+  
+substituteDL :: [DataLayout BitRange] -> DataLayout' BitRange -> DataLayout' BitRange
+substituteDL ls l = case l of
+  VarLayout n s -> case ls !! (natToInt n) of
+                   CLayout -> __impossible "substituteS in Inference: CLayout shouldn't be here"
+                   Layout l -> offset s l
+  SumLayout tag alts ->
+    let altl = M.toList alts
+        fns = fmap fst altl
+        fis = fmap fst $ fmap snd altl
+        fes = fmap snd $ fmap snd altl
+     in SumLayout tag $ M.fromList (zip fns $ zip fis (fmap (substituteDL ls) fes))
+  RecordLayout fs ->
+    let fsl = M.toList fs
+        fns = fmap fst fsl
+        fes = fmap snd fsl
+     in RecordLayout $ M.fromList (zip fns (fmap (substituteDL ls) fes))
 #ifdef BUILTIN_ARRAYS
-      ArrayLayout e -> ArrayLayout $ substituteS' ls e
+  ArrayLayout e -> ArrayLayout $ substituteDL ls e
 #endif
-      _ -> l
+  _ -> l
 
 substituteLE :: Vec t (Type u b) -> LExpr t b -> LExpr u b
 substituteLE vs = \case
@@ -292,8 +292,7 @@ adjust k f = map (\(a,b) -> (a,) $ if a == k then f b else b)
 newtype TC (t :: Nat) (v :: Nat) b x
   = TC {unTC :: ExceptT String
                         (ReaderT (Vec t Kind, Map FunName (FunctionType b))
-                                 (State ( Vec v (Maybe (Type t b))
-                                        , [(DataLayout' BitRange, Type t b)] )))
+                                 (State (Vec v (Maybe (Type t b)))))
                         x}
   deriving (Functor, Applicative, Alternative, Monad, MonadPlus,
             MonadReader (Vec t Kind, Map FunName (FunctionType b)))
@@ -343,21 +342,21 @@ opType Complement [TPrim p] | p /= Boolean = Just $ TPrim p
 opType opr ts = __impossible "opType"
 
 useVariable :: Fin v -> TC t v b (Maybe (Type t b))
-useVariable v = TC $ do ret <- (`at` v) <$> use _1
+useVariable v = TC $ do ret <- (`at` v) <$> get
                         case ret of
                           Nothing -> return ret
                           Just t  -> do
                             ok <- canShare <$> unTC (kindcheck t)
-                            unless ok $ modify (\(s1,s2) -> (,s2) $ update s1 v Nothing)
+                            unless ok $ modify (\s -> update s v Nothing)
                             return ret
 
 funType :: CoreFunName -> TC t v b (Maybe (FunctionType b))
-funType v = TC $ M.lookup (unCoreFunName v) . snd <$> ask
+funType v = TC $ (M.lookup (unCoreFunName v) . snd) <$> ask
 
 runTC :: TC t v b x
       -> (Vec t Kind, Map FunName (FunctionType b))
-      -> (Vec v (Maybe (Type t b)), [(DataLayout' BitRange, Type t b)])
-      -> Either String ((Vec v (Maybe (Type t b)), [(DataLayout' BitRange, Type t b)]) , x)
+      -> Vec v (Maybe (Type t b))
+      -> Either String (Vec v (Maybe (Type t b)), x)
 runTC (TC a) readers st = case runState (runReaderT (runExceptT a) readers) st of
                             (Left x, s)  -> Left x
                             (Right x, s) -> Right (s,x)
@@ -391,40 +390,155 @@ tc = flip tc' M.empty
     tc' [] reader = return ([], reader)
     tc' ((FunDef attr fn ks ls t rt e):ds) reader =
       -- Enable recursion by inserting this function's type into the function type dictionary
-      let c0 = zip (fmap (`VarLayout` 0) [Zero ..]) $ Vec.cvtToList ls <&> (^._2)
-          ft = FT (snd <$> ks) (Vec.length ls) c0 t rt in
-      case runTC (infer e >>= flip typecheck rt) (fmap snd ks, M.insert fn ft reader) (Cons (Just t) Nil, c0) of
+      let ft = FT (snd <$> ks) (Vec.length ls) [] t rt in
+      case runTC (infer e >>= flip typecheck rt) (fmap snd ks, M.insert fn ft reader) (Cons (Just t) Nil) of
         Left x -> Left x
-        Right ((_,c), e') -> first (FunDef attr fn ks ls t rt e':) <$> tc' ds (M.insert fn (FT (fmap snd ks) (Vec.length ls) c t rt) reader)
-    tc' (d@(AbsDecl _ fn ks ls t rt):ds) reader = 
+        Right (_, e') ->
+           let c0 = zip (fmap (`VarLayout` 0) [Zero ..]) $ Vec.cvtToList ls <&> (^._2) in
+           let cls = nub $ inferLayConstraints t ++ inferLayConstraints rt ++ inferLayConstraintsTE reader e' ++ c0 in
+           let m = (M.insert fn (FT (fmap snd ks) (Vec.length ls) cls t rt) reader) in
+           
+             (first (FunDef attr fn ks ls t rt e':)) <$> tc' ds m
+    tc' (d@(AbsDecl _ fn ks ls t rt):ds) reader =
+      let cls = nub $ 
+            (zip (fmap (`VarLayout` 0) [Zero ..]) $ Vec.cvtToList ls <&> (^._2))
+            ++ inferLayConstraints t ++  inferLayConstraints rt 
+      in      
       first (Unsafe.unsafeCoerce d:) <$>
-        tc' ds (M.insert fn (FT (fmap snd ks) (Vec.length ls) (zip (fmap (`VarLayout` 0) [Zero ..]) $ Vec.cvtToList ls <&> (^._2)) t rt) reader)
-    tc' (d:ds) reader = first (Unsafe.unsafeCoerce d:) <$> tc' ds reader
+        tc' ds (M.insert fn (FT (fmap snd ks) (Vec.length ls) cls t rt) reader)
+    tc' (d:ds) reader = (first (Unsafe.unsafeCoerce d:)) <$> tc' ds reader
 
 tc_ :: (Show b, Eq b, Pretty b, a ~ b)
     => [Definition UntypedExpr a b]
     -> Either String [Definition TypedExpr a b]
 tc_ = fmap fst . tc
 
+isMonoType :: Type t b -> Bool
+isMonoType (TVar _) = False
+isMonoType (TVarBang _) = False
+isMonoType (TVarUnboxed _) = False
+isMonoType (TCon _ l _) = all isMonoType l
+isMonoType (TFun t rt) = isMonoType t && isMonoType rt
+isMonoType (TPrim _) = True
+isMonoType TString = True
+isMonoType (TSum l) = all (isMonoType . fst . snd) l
+isMonoType (TProduct t1 t2) = isMonoType t1 && isMonoType t2
+isMonoType (TRecord _ fs _) = all (isMonoType . fst . snd) fs     
+isMonoType TUnit = True
+isMonoType (TRPar _ _)  = True -- TODO (not sure if something must be done)
+isMonoType (TRParBang _ _) = True -- TODO (not sure if something must be done)
+-- #ifdef BUILTIN_ARRAYS
+isMonoType (TArray t _ s _) = isMonoType t -- TODO
+isMonoType (TRefine t _) = isMonoType t -- TODO
+-- #endif
+
+isMonoDataLayout' :: DataLayout' BitRange -> Bool
+isMonoDataLayout' UnitLayout = True
+isMonoDataLayout' (PrimLayout b) = True
+isMonoDataLayout' (RecordLayout fs) = all isMonoDataLayout' fs  
+isMonoDataLayout' (SumLayout tag alts) = all (isMonoDataLayout' . snd) alts
+isMonoDataLayout' (VarLayout v offset) = False
+#ifdef BUILTIN_ARRAYS
+isMonoDataLayout' (ArrayLayout l) = isMonoDataLayout' l
+#endif
+
+
+-- TODO ne garder que les types/data layouts pas clos
+inferLayConstraints :: Type t b -> [(DataLayout' BitRange, Type t b)]
+inferLayConstraints (TVar _) = []
+inferLayConstraints (TVarBang _) = []
+inferLayConstraints (TVarUnboxed _) = []
+inferLayConstraints (TCon _ l _) = concatMap inferLayConstraints l
+inferLayConstraints (TFun t rt) = inferLayConstraints t ++ inferLayConstraints rt
+inferLayConstraints (TPrim _) = []
+inferLayConstraints TString = []
+inferLayConstraints (TSum l) = concatMap (inferLayConstraints . fst . snd) l
+inferLayConstraints (TProduct t1 t2) = inferLayConstraints t1 ++ inferLayConstraints t2
+inferLayConstraints (TRecord r fs s) =    
+    let cs = concatMap (inferLayConstraints . fst . snd) fs in
+    case s of
+      Boxed _ (Layout l) ->
+            if isMonoDataLayout' l && all (isMonoType . fst . snd) fs then 
+                cs
+            else
+                (l, TRecord r fs Unboxed) : cs
+      _ -> cs
+inferLayConstraints TUnit = []
+inferLayConstraints (TRPar _ _)  = [] -- TODO (not sure if something must be done)
+inferLayConstraints (TRParBang _ _) = [] -- TODO (not sure if something must be done)
+-- #ifdef BUILTIN_ARRAYS
+inferLayConstraints (TArray t _ s _) = [] -- TODO
+inferLayConstraints (TRefine t _) = inferLayConstraints t
+-- #endif
+
+inferLayConstraintsTE :: Map FunName (FunctionType a) -> TypedExpr t v a a -> [(DataLayout' BitRange, Type t a)]
+inferLayConstraintsTE m (TE t e) = inferLayConstraintsTE' m e ++ inferLayConstraints t
+
+
+
+inferLayConstraintsTE' :: Map FunName (FunctionType a) -> Expr t v a a TypedExpr -> [(DataLayout' BitRange, Type t a)]
+inferLayConstraintsTE' m (Variable _) = []
+inferLayConstraintsTE' m (Fun f ts ls note) 
+   | ExI (Flip ts') <- Vec.fromList ts  
+   = 
+        case M.lookup (unCoreFunName f) m of
+          Just (FT ks nl lts _ _) ->
+             case Vec.length ts' =? Vec.length ks
+               of Just Refl ->
+                     concatMap inferLayConstraints ts ++                         
+                          map (substituteDL ls *** (substitute ts' . substituteL ls)) lts            
+          _        -> error $ "Something went wrong in lookup of function type: '" ++ unCoreFunName f ++ "'"
+inferLayConstraintsTE' m (Op _ l) = concatMap (inferLayConstraintsTE m) l
+inferLayConstraintsTE' m (Con _ _ t) = inferLayConstraints t
+inferLayConstraintsTE' m Unit = []
+inferLayConstraintsTE' m (ILit _ _) = []
+inferLayConstraintsTE' m (SLit _) = []
+#ifdef BUILTIN_ARRAYS
+inferLayConstraintsTE' m (ALit l) = concatMap (inferLayConstraintsTE m) l
+inferLayConstraintsTE' m (ArrayIndex t u) = concatMap (inferLayConstraintsTE m) [t, u]
+inferLayConstraintsTE' m (Pop _ t u) = concatMap (inferLayConstraintsTE m) [t, u]
+inferLayConstraintsTE' m (Singleton t) = inferLayConstraintsTE t
+-- TODO check de Bruijn indices
+inferLayConstraintsTE' m (ArrayMap2 (_, e1) (e2, e3) = concatMap (inferLayConstraintsTE m) [e1, e2, e3]
+inferLayConstraintsTE' m (ArrayTake _ e1 e2 e3) =  concatMap (inferLayConstraintsTE m) [e1, e2, e3]
+inferLayConstraintsTE' m (ArrayPut _ e2 e3) =  concatMap (inferLayConstraintsTE m) [e1, e2, e3]
+#endif
+-- TODO check de Bruijn indices
+inferLayConstraintsTE' m (Let _ t u) = inferLayConstraintsTE m t ++ inferLayConstraintsTE m u
+inferLayConstraintsTE' m (LetBang _ _ t u) = inferLayConstraintsTE m t ++ inferLayConstraintsTE m u
+inferLayConstraintsTE' m (Tuple t u) = inferLayConstraintsTE m t ++ inferLayConstraintsTE m u 
+inferLayConstraintsTE' m (Struct l) = concatMap (inferLayConstraintsTE m . snd) l
+inferLayConstraintsTE' m (If e1 e2 e3) =  concatMap (inferLayConstraintsTE m) [e1, e2, e3]
+inferLayConstraintsTE' m (Case e1 _ (_, _, e2) (_, _, e3)) = 
+      inferLayConstraintsTE m e1 ++ inferLayConstraintsTE m e2 ++ inferLayConstraintsTE m e3
+inferLayConstraintsTE' m (Esac t) = inferLayConstraintsTE m t
+inferLayConstraintsTE' m (Split _ e1 e2) = inferLayConstraintsTE m e1 ++ inferLayConstraintsTE m e2
+inferLayConstraintsTE' m (Member e _) =  inferLayConstraintsTE m e
+inferLayConstraintsTE' m (Take _ e1 _ e2) = inferLayConstraintsTE m e1 ++ inferLayConstraintsTE m e2
+inferLayConstraintsTE' m (Put e1 _ e2) =  concatMap (inferLayConstraintsTE m) [e1, e2]
+inferLayConstraintsTE' m (Promote t e) = inferLayConstraints t ++ inferLayConstraintsTE m e
+inferLayConstraintsTE' m (Cast t e) = inferLayConstraints t ++ inferLayConstraintsTE m e
+inferLayConstraintsTE' m (App t u) =  inferLayConstraintsTE m t ++ inferLayConstraintsTE m u 
+
 tcConsts :: [CoreConst UntypedExpr]
          -> Map FunName (FunctionType VarName)
          -> Either String ([CoreConst TypedExpr], Map FunName (FunctionType VarName))
 tcConsts [] reader = return ([], reader)
 tcConsts ((v,e):ds) reader =
-  case runTC (infer e) (Nil, reader) (Nil, []) of
+  case runTC (infer e) (Nil, reader) Nil of
     Left x -> Left x
-    Right (_,e') -> first ((v,e'):) <$> tcConsts ds reader
+    Right (_,e') -> (first ((v,e'):)) <$> tcConsts ds reader
 
 withBinding :: Type t b -> TC t ('Suc v) b x -> TC t v b x
 withBinding t x
   = TC $ do readers <- ask
             st      <- get
-            case runTC x readers (first (Cons $ Just t) st) of
+            case runTC x readers (Cons (Just t) st) of
               Left e -> throwError e
-              Right ((Cons Nothing  s, c), r) -> do put (s,c); return r
-              Right ((Cons (Just t) s, c), r) -> do
+              Right (Cons Nothing s,r)   -> do put s; return r
+              Right (Cons (Just t) s, r) -> do
                 ok <- canDiscard <$> unTC (kindcheck t)
-                if ok then put (s,c) >> return r
+                if ok then put s >> return r
                       else throwError "Didn't use linear variable"
 
 withBindings :: Vec k (Type t b) -> TC t (v :+: k) b x -> TC t v b x
@@ -432,10 +546,10 @@ withBindings Nil tc = tc
 withBindings (Cons x xs) tc = withBindings xs (withBinding x tc)
 
 withBang :: [Fin v] -> TC t v b x -> TC t v b x
-withBang vs (TC x) = TC $ do st <- use _1
-                             mapM_ (\v -> _1 %= modifyAt v (fmap bang)) vs
+withBang vs (TC x) = TC $ do st <- get
+                             mapM_ (\v -> modify (modifyAt v (fmap bang))) vs
                              ret <- x
-                             mapM_ (\v -> _1 %= modifyAt v (const $ st `at` v)) vs
+                             mapM_ (\v -> modify (modifyAt v (const $ st `at` v))) vs
                              return ret
 
 lookupKind :: Fin t -> TC t v b Kind
@@ -560,7 +674,8 @@ infer (E (Variable v))
 infer (E (Fun f ts ls note))
    | ExI (Flip ts') <- Vec.fromList ts
    , ExI (Flip ls') <- Vec.fromList ls
-   = do x <- funType f
+   = do myMap <- ask
+        x <- funType f
         case x of
           Just (FT ks nl lts ti to) ->
             case (Vec.length ts' =? Vec.length ks, Vec.length ls' =? nl)
